before list change

VCVio/OracleComp/Constructions/Replicate.lean
@@ -3,13 +3,13 @@ Copyright (c) 2024 Devon Tuma. All rights reserved.
 Released under Apache 2.0 license as described in the file LICENSE.
 Authors: Devon Tuma
 -/
-import VCVio.OracleComp.DistSemantics.EvalDist
+import VCVio.OracleComp.Constructions.UniformSelect
 
 /-!
 # Running a Computation Multiple Times
 
 This file defines a function `replicate oa n` that runs the computation `oa` a total of `n` times,
-returning the result as a vector of length `n`.
+returning the result as a list of length `n`.
 
 Note that while the executions are independent, they may no longer be after calling `simulate`.
 -/
@@ -20,32 +20,35 @@ namespace OracleComp
 
 variable {spec : OracleSpec} {α β : Type}
 
-/-- Run the computation `oa` `n` times to get a `Vector α n` -/
-def replicate (oa : OracleComp spec α) (n : ℕ) : OracleComp spec (Vector α n) :=
+/-- Run the computation `oa` repeatedly `n` times to get a list of `n` results. -/
+def replicate (oa : OracleComp spec α) (n : ℕ) : OracleComp spec (List α) :=
     match n with
-    | 0 => return Vector.nil
-    | (n + 1) => (· ::ᵥ ·) <$> oa <*> replicate oa n
+    | 0 => return []
+    | (n + 1) => (· :: ·) <$> oa <*> replicate oa n
+
+def replicateVec (oa : OracleComp spec α) (n : ℕ) : OracleComp spec (Vector α n) :=
+    (λ xs ↦ Vector.ofFn (λ i ↦ if h : ↑i < xs.length then xs[i]'h else oa.defaultResult))
+        <$> replicate oa n
 
 @[simp low]
-lemma replicate_zero (oa : OracleComp spec α) : oa.replicate 0 = pure Vector.nil := rfl
+lemma replicate_zero (oa : OracleComp spec α) : oa.replicate 0 = return [] := rfl
 
 @[simp low]
 lemma replicate_succ (oa : OracleComp spec α) (n : ℕ) :
-    oa.replicate (n + 1) = (· ::ᵥ ·) <$> oa <*> replicate oa n := rfl
-
--- @[simp]
--- lemma replicate_add (oa : OracleComp spec α) (n m : ℕ) :
---         (replicate oa (n + m)) = (· ++ ·) <$> replicate oa n <*> replicate oa m := by
---     induction n with
---     | zero => simp only [Nat.zero_eq, zero_add, replicate_zero,
---         map_pure, List.nil_append, pure_id'_seq]
---     | succ n hn => simp only [Nat.succ_add, replicate_succ, map_eq_bind_pure_comp,
---         Function.comp, hn, seq_eq_bind, bind_assoc, pure_bind, List.cons_append]
+    oa.replicate (n + 1) = (· :: ·) <$> oa <*> replicate oa n := rfl
 
 @[simp]
-lemma probOutput_replicate (oa : OracleComp spec α) (n : ℕ) (xs : Vector α n) :
-        [= xs | replicate oa n] =  (xs.toList.map ([= · | oa])).prod := by
-        --if xs.length = n then (xs.map ([= · | oa])).prod else 0 := by
+lemma replicate_add (oa : OracleComp spec α) (n m : ℕ) :
+        (replicate oa (n + m)) = (· ++ ·) <$> replicate oa n <*> replicate oa m := by
+    induction n with
+    | zero => simp only [Nat.zero_eq, zero_add, replicate_zero,
+        map_pure, List.nil_append, pure_id'_seq]
+    | succ n hn => simp only [Nat.succ_add, replicate_succ, map_eq_bind_pure_comp,
+        Function.comp, hn, seq_eq_bind, bind_assoc, pure_bind, List.cons_append]
+
+@[simp]
+lemma probOutput_replicate (oa : OracleComp spec α) (n : ℕ) (xs : List α) :
+        [= xs | replicate oa n] = if xs.length = n then (xs.map ([= · | oa])).prod else 0 := by
     induction n with
     | zero => {
         sorry
@@ -60,7 +63,15 @@ lemma probOutput_replicate (oa : OracleComp spec α) (n : ℕ) (xs : Vector α n
 
 @[simp]
 lemma support_replicate (oa : OracleComp spec α) (n : ℕ) :
-        (replicate oa n).support = {xs | ∀ x ∈ xs.toList, x ∈ oa.support} := by
+        (replicate oa n).support = {xs | ∀ x ∈ xs, x ∈ oa.support} := by
     sorry
+
+/-- Vectors can be selected uniformly if the underlying type can be.
+Note: this isn't very efficient as an actual implementation in practice. -/
+instance (α : Type) [Fintype α] [Inhabited α] [SelectableType α] (n : ℕ) :
+    SelectableType (Vector α n) where
+  selectElem := (λ xs ↦ Vector.ofFn (λ i ↦ if h : ↑i < xs.length then xs[i]'h else default))
+        <$> replicate ($ᵗ α) n
+  probOutput_selectElem := sorry
 
 end OracleComp
